source/proof.v
@@ -1,5 +1,5 @@
 
-From S5 Require Export set.
+From S5 Require Export form.
 
 Fixpoint interpret (f : form) (m : model) (w : m) : Prop :=
   match f with
@@ -9,14 +9,14 @@ Fixpoint interpret (f : form) (m : model) (w : m) : Prop :=
   | Box f => forall (v : m), rel w v -> interpret f m v
   end.
 
-Inductive ax_s5 : set -> set :=
-  | a_0 (G : set) (f : form) : G f -> ax_s5 G f
-  | a_1 (G : set) (f g : form) : ax_s5 G (Impl f (Impl g f))
-  | a_2 (G : set) (f g h : form) : ax_s5 G (Impl (Impl f (Impl g h)) (Impl (Impl f g) (Impl f h)))
-  | a_3 (G : set) (f g : form) : ax_s5 G (Impl (Impl (Neg f) (Neg g)) (Impl g f))
-  | a_k (G : set) (f g : form) : ax_s5 G (Impl (Box (Impl f g)) (Impl (Box f) (Box g)))
-  | a_t (G : set) (f : form) : ax_s5 G (Impl (Box f) f)
-  | a_4 (G : set) (f : form) : ax_s5 G (Impl (Box f) (Box (Box f)))
-  | a_b (G : set) (f : form) : ax_s5 G (Impl f (Box (Diamond f)))
-  | mp (G : set) (f g : form) : ax_s5 G (Impl f g) -> ax_s5 G f -> ax_s5 G g
-  | nec (G : set) (f : form) : ax_s5 empty_set f -> ax_s5 G (Box f).
+Inductive ax_s5 : form_set -> form_set :=
+  | a_0 (G : form_set) (f : form) : G f -> ax_s5 G f
+  | a_1 (G : form_set) (f g : form) : ax_s5 G (Impl f (Impl g f))
+  | a_2 (G : form_set) (f g h : form) : ax_s5 G (Impl (Impl f (Impl g h)) (Impl (Impl f g) (Impl f h)))
+  | a_3 (G : form_set) (f g : form) : ax_s5 G (Impl (Impl (Neg f) (Neg g)) (Impl g f))
+  | a_k (G : form_set) (f g : form) : ax_s5 G (Impl (Box (Impl f g)) (Impl (Box f) (Box g)))
+  | a_t (G : form_set) (f : form) : ax_s5 G (Impl (Box f) f)
+  | a_4 (G : form_set) (f : form) : ax_s5 G (Impl (Box f) (Box (Box f)))
+  | a_b (G : form_set) (f : form) : ax_s5 G (Impl f (Box (Diamond f)))
+  | mp (G : form_set) (f g : form) : ax_s5 G (Impl f g) -> ax_s5 G f -> ax_s5 G g
+  | nec (G : form_set) (f : form) : ax_s5 empty_set f -> ax_s5 G (Box f).
