source/set.v
@@ -1,31 +1,42 @@
 
-From S5 Require Export form.
+Section set.
 
-Definition set := form -> Prop.
+  Variable T : Type.
 
-Definition empty_set : set := 
-  fun (f : form) => False.
+  Definition set T := T -> Prop.
 
-Definition subset (F G : set) : Prop :=
-  forall x, F x -> G x.
+  Definition empty_set : set T := 
+    fun (f : T) => False.
 
-Definition add_singleton (G : set) (f : form) : set :=
-  fun x => x = f \/ G x.
+  Definition subset (F G : set T) : Prop :=
+    forall x, F x -> G x.
 
-Lemma subset_lemma (F G : set) (f : form) :
-  subset F G -> F f -> G f.
-Proof.
-  intros H Ff. apply H, Ff.
-Qed.
+  Definition add_singleton (G : set T) (a : T) : set T :=
+    fun x => x = a \/ G x.
+  
+  Lemma subset_lemma (F G : set T) (a : T) :
+  subset F G -> F a -> G a.
+  Proof.
+    intros H Ff. apply H, Ff.
+  Qed.
 
-Lemma member_add_singleton (G : set) (f : form) :
-  (add_singleton G f) f.
-Proof. 
-  unfold add_singleton. left. reflexivity.
-Qed.
+  Lemma subset_add_singleton (G : set T) (a : T) :
+    subset G (add_singleton G a).
+  Proof.
+    intros g Gg. unfold add_singleton. right. assumption.
+  Qed.
 
-Lemma subset_add_singleton (G : set) (f : form) :
-  subset G (add_singleton G f).
-Proof.
-  intros g Gg. unfold add_singleton. right. assumption.
-Qed.
+  Lemma member_add_singleton (G : set T) (a : T) :
+    (add_singleton G a) a.
+  Proof. 
+    unfold add_singleton. left. reflexivity.
+  Qed.
+
+End set.
+
+Arguments empty_set {_}.
+Arguments subset {_} F G.
+Arguments add_singleton {_} G a.
+Arguments subset_lemma {_} F G a.
+Arguments subset_add_singleton {_} G a.
+Arguments member_add_singleton {_} G a.
