source/deduce.v
@@ -1,7 +1,7 @@
 
 From S5 Require Export inference.
 
-Lemma ax_s5_subset (F G : set) (f : form) :
+Lemma ax_s5_subset (F G : form_set) (f : form) :
   ax_s5 F f -> subset F G -> ax_s5 G f.
 Proof.
   intros H1 H2. induction H1.
@@ -19,7 +19,7 @@ Proof.
   - apply nec. assumption.
 Qed.
 
-Lemma deduction_theorem_1 (G : set) (f g : form) :
+Lemma deduction_theorem_1 (G : form_set) (f g : form) :
   ax_s5 G (Impl f g) -> ax_s5 (add_singleton G f) g.
 Proof.
   intros H0. eapply mp.
@@ -29,7 +29,7 @@ Proof.
   - apply a_0, member_add_singleton.
 Qed.
 
-Lemma deduction_theorem_2 (G : set) (f g : form) :
+Lemma deduction_theorem_2 (G : form_set) (f g : form) :
   ax_s5 (add_singleton G f) g -> ax_s5 G (Impl f g).
 Proof.
   intros H. remember (add_singleton G f) as G'. induction H; subst.
@@ -51,7 +51,7 @@ Proof.
   - eapply mp. apply a_1. apply nec, H.
 Qed.
 
-Lemma deduction_theorem (G : set) (f g : form) :
+Lemma deduction_theorem (G : form_set) (f g : form) :
   ax_s5 G (Impl f g) <-> ax_s5 (add_singleton G f) g.
 Proof.
   split.
